common/theories/Notes.md
@@ -5,6 +5,33 @@
 
 # Notes ajout condition
 
+  This must be well-formed:
+
+    ↓↓g_args ,,, ↓g_largs ,,,  (↓σ)(l_nuparams ,,, indices)
+
+    1. rc_notin args
+    2. rc_notin largs
+    3. σ must **not** well-formed, but its subtitution yes.
+       As isup_notin (l_nuparams ,,, indices) => only care about not-isup
+       (bit more flexible)
+
+    Addition of 2. and 3. to positivity forces us to prove it in
+    1. sub_uprams:
+        the instantiation to substitute is nested => get sth nested i.e. stuff to prove
+        needed it for uparams case
+    2. specialize_argument:
+
+        forall (i : nat) (x : term),
+        rc_notin_bool (map check_lax Γ) (i + nb_binders) x ->
+        rc_notin_bool (map check_lax (args ++ l_args + nuparams ++ mapi_rec specialize_argument Γ nb_l_nuparams))
+        (i + nb_binders) x.[up (i + (nb_l_nuparams + #|Γ| + nb_binders)) inst_uparams]
+
+    should work, no ?
+    args true peut venir que de σ:
+    opt 1. => rc_notin σ donc ok => prendre just args_no_rc ? => vie plus simple
+    ? opt 2. => isup notin ? => σ not isup => rc_notin donc ok
+
+
 1. is check_lax arg = true -> rc_notin ok ?
 2. Do I really needs to extra-conditions ?
 3. What about cstr_extra_args needing to be false ?
